Tested SemOp to examples; it seems work

examples/ProcDecSC.v
@@ -1,7 +1,7 @@
 Require Import Bool String List.
 Require Import Lib.CommonTactics Lib.ilist Lib.Word Lib.Struct Lib.StringBound Lib.FMap.
 Require Import Lts.Syntax Lts.Semantics Lts.Equiv Lts.Refinement Lts.Renaming.
-Require Import Lts.Decomposition Lts.Renaming Lts.Inline Lts.InlineFacts_2.
+Require Import Lts.Decomposition Lts.Renaming Lts.Inline Lts.InlineFacts_2 Lts.SemOp.
 Require Import Ex.SC Ex.Fifo Ex.MemAtomic Ex.ProcDec.
 
 Set Implicit Arguments.
@@ -16,23 +16,148 @@ Section ProcDecSC.
 
   Definition pdecN := procDecM fifoSize dec exec n.
   Definition scN := sc dec exec opLd opSt opHt n.
-  Hint Unfold pdecN scN : ModuleDefs.
 
   Section SingleCore.
     Definition pdec := pdecf fifoSize dec exec.
     Definition pinst := pinst dec exec opLd opSt opHt.
-    Hint Unfold pdec pinst.
+
+    Definition pdec_pinst_ruleMap (_: RegsT) (s: string): option string :=
+      if string_dec s "reqLd" then None
+      else if string_dec s "reqSt" then None
+      else if string_dec s "repLd" then None
+      else if string_dec s "repSt" then None
+      else if string_dec s "execHt" then Some "execHt"%string
+      else if string_dec s "execNm" then Some "execNm"%string
+      else if string_dec s "processLd" then Some "execLd"%string
+      else if string_dec s "processSt" then Some "execSt"%string
+      else None.
+
+    (* Eval vm_compute in (getRegInits pdec). *)
+    (* = ["pc"%string; "rf"%string; "stall"%string; "Ins.elt"%string; "Ins.enqP"%string; *)
+    (*    "Ins.deqP"%string; "Ins.empty"%string; "Ins.full"%string; "Outs.elt"%string; *)
+    (*    "Outs.enqP"%string; "Outs.deqP"%string; "Outs.empty"%string; "Outs.full"%string] *)
+    (*   : list string *)
+    
+    Definition pdec_pinst_regMap (r: RegsT): RegsT.
+    Proof.
+      destruct (M.find "pc"%string r) as [[pck pcv]|]; [|exact (M.empty _)].
+      destruct pck as [pck|]; [|exact (M.empty _)].
+      destruct (decKind pck (Bit addrSize)); [subst|exact (M.empty _)].
+      
+      destruct (M.find "rf"%string r) as [[rfk rfv]|]; [|exact (M.empty _)].
+      destruct rfk as [rfk|]; [|exact (M.empty _)].
+      destruct (decKind rfk (Vector (Bit valSize) rfIdx)); [subst|exact (M.empty _)].
+      
+      destruct (M.find "Outs.empty"%string r) as [[oek oev]|]; [|exact (M.empty _)].
+      destruct oek as [oek|]; [|exact (M.empty _)].
+      destruct (decKind oek Bool); [subst|exact (M.empty _)].
+
+      destruct (M.find "Outs.elt"%string r) as [[oelk oelv]|]; [|exact (M.empty _)].
+      destruct oelk as [oelk|]; [|exact (M.empty _)].
+      destruct (decKind oelk (Vector (memAtomK addrSize valSize) fifoSize));
+        [subst|exact (M.empty _)].
+
+      destruct (M.find "Outs.deqP"%string r) as [[odk odv]|]; [|exact (M.empty _)].
+      destruct odk as [odk|]; [|exact (M.empty _)].
+      destruct (decKind odk (Bit fifoSize)); [subst|exact (M.empty _)].
+      
+      refine (if oev then _ else _).
+
+      - refine (M.add "pc"%string _
+                      (M.add "rf"%string _
+                             (M.empty _))).
+        + exact (existT _ _ pcv).
+        + exact (existT _ _ rfv).
+
+      - refine (M.add "pc"%string _
+                      (M.add "rf"%string _
+                             (M.empty _))).
+        + exact (existT _ _ (getNextPc exec _ pcv rfv (dec _ rfv pcv))).
+        + pose proof (dec _ rfv pcv ``"opcode") as opc.
+          destruct (weq opc (evalConstT opLd)).
+          * refine (existT _ (SyntaxKind (Vector (Bit valSize) rfIdx)) _); simpl.
+            exact (fun a => if weq a (dec _ rfv pcv ``"reg")
+                            then (oelv odv) ``"value"
+                            else rfv a).
+          * refine (existT _ _ rfv).
+    Defined.
+
+    Ltac dest_rules :=
+      repeat
+        match goal with
+        | [H: In _ _ |- _] => inv H
+        | [H: (_ :: _)%struct = (_ :: _)%struct |- _] => inv H
+        end.
+    
+    Lemma attribute_invert:
+      forall {k: Type} n1 n2 (a1 a2: k),
+        (n1 :: a1)%struct = (n2 :: a2)%struct -> a1 = a2.
+    Proof. intros; inv H; auto. Qed.
+
+    Ltac invert_call :=
+      (* Figure out if the call is internal or not *)
+      repeat
+        match goal with
+        | [H: (_ /\ _) \/ (_ /\ _) |- _] => destruct H; dest; subst; simpl in *
+        | [H: ~ (_ \/ _) |- _] => try (elim H; tauto; fail)
+        end;
+      (* Find the call body *)
+      repeat
+        match goal with
+        | [H: ((_ :: _)%struct = (_ :: _)%struct \/ _) |- _] => destruct H 
+        | [H: (_ :: _)%struct = (_ :: _)%struct |- _] =>
+          try (inv H; fail);
+          try (apply attribute_invert in H; destruct_existT)
+        | [H: False |- _] => elim H
+        end.
 
     Lemma pdec_refines_pinst: pdec <<== pinst.
     Proof.
-      admit.
-    Qed.
+      apply stepRefinement with (ruleMap:= pdec_pinst_ruleMap) (theta:= pdec_pinst_regMap);
+        [admit (* cannot use computation because of parameters... *)|].
+
+      intros.
+      apply step_implies_StepOp in H.
+      exists (pdec_pinst_regMap u).
+      rewrite idElementwiseId.
+
+      assert (forall o u l iics,
+                 SubstepOp pdec o u l iics ->
+                 exists sics,
+                   SubstepOp pinst (pdec_pinst_regMap o) (pdec_pinst_regMap u)
+                             (liftPLabel id pdec_pinst_ruleMap o l)
+                             sics).
+      { clear; intros; eexists.
+        inv H; [exfalso; admit|exfalso; admit| |]. (* two admits; trivial empty cases *)
+
+        - dest_rules.
+          + invertActionOpRep.
+            invert_call.
+            invertActionOpRep.
+            apply SSSEmptyRule; auto.
+
+          + invertActionOpRep.
+            invert_call.
+            invertActionOpRep.
+            apply SSSEmptyRule; auto.
+
+          + admit.
+          + admit.
+          + admit.
+          + admit.
+          + admit.
+          + admit.
+
+        - admit. (* meths case *)
+      }
+
+    Abort.
 
   End SingleCore.
 
-  Lemma pdecN_refines_scN: pdecN <<== scN.
+  Lemma pdecN_refines_scN: traceRefines id pdecN scN.
   Proof.
-    admit.
+    apply traceRefines_modular_interacting with (vp:= (@idElementwise _)); admit.
   Qed.
 
 End ProcDecSC.
